analysis/facts/behavior/schedule.v
@@ -1,0 +1,31 @@
+Require Export prosa.util.all.
+Require Export prosa.behavior.all.
+
+(** * Schedules *)
+
+(** In this file, we establish basic facts about the jobs scheduled in a given
+    processor state, i.e., about the generic notions derived from [job_on]. *)
+
+Section ScheduledJobs.
+
+  (** Consider any type of jobs, ... *)
+  Context {Job : JobType}.
+
+  (** ... and any type of processor state. *)
+  Context {PState : ProcessorState Job}.
+
+  (** We observe that a job is scheduled in a given processor state exactly if it
+      occurs in the list of jobs scheduled in that state. That is, the predicate
+      [scheduled_in] and the enumeration [jobs_scheduled_in] agree. *)
+  Lemma jobs_scheduled_in_iff :
+    forall (j : Job) (s : PState),
+      scheduled_in j s = (j \in jobs_scheduled_in s).
+  Proof.
+    move=> j s; apply/idP/idP.
+    - move=> /existsP[c /eqP ON].
+      by rewrite /jobs_scheduled_in mem_pmap -ON map_f ?mem_enum.
+    - rewrite /jobs_scheduled_in mem_pmap => /mapP[c _ EQ].
+      by apply/existsP; exists c; rewrite /scheduled_on -EQ.
+  Qed.
+
+End ScheduledJobs.
